# Javascript
```js
function f(l){
	e = []
	d = 0
	for(x in l){
		if(d) {
			f = l[x]-d
			e.push(f>0?"+"+f:f)
		}
		d = l[x]
	}
	throw ' /'+e.join('\\ /')+"\\\n"+l.join("    ")
}
```

# Python
```py
def f(l):
    d = []
    for i in range(len(l)-1):
        d.append(l[i+1] - l[i])
    x = ''
    y = ''
    for i in range(len(l)-1):
        z = str(l[i])
        w = str(d[i])
        if w[0] != '-':
            w = '+' + w
        x += ' ' * len(z) + '/' + w + '\\'
        y += z + 2 * ' ' + len(w) * ' '
    y += str(l[-1])
    z = 'spong,ebob'
    print(x + '\n' + y)
```

```py
def f(l):
   a=''
   b=''
   for i in range(len(l)-1):
    s=''
    f=str(l[i])
    r=l[i+1]-l[i]
    if (r > 0):
      s='+'
    a+= ' ' * len(f) + '/' + s +str(r) + '\\'
    b+= f + ' '*(len('/'+ s + str(r) +'\\'))
   z = 'spong,ebob'
   print a + '\n' + b + str(l[-1])
```

# Ruby
```rb
def f(bob)
  spo, nge = " ", ""

  bob.each_cons(2) { |s|
    r = s[1] - s[0]
    spo << t = "/#{r > 0 ? "+" << r.to_s : r}\\" + " " * s[1].to_s.length
    nge << s[0].to_s + " " * (t.length - 1)
  }
  nge << bob.last
  puts spo
  print nge 
  puts bob.last
end
```